src/CFG/Compiler/Compile_Certificate.thy
@@ -110,18 +110,23 @@ proof (intro allI impI)
     cb: "compile \<Pi> p (body decl) (Statement (m + csize (body decl))) m
            = (m + csize (body decl), Statement m, Eb, Kf)"
     and Edef: "Ef = insert (FunctionEntry p, EA_Nop, Statement m)
-                 (insert (Statement (m + csize (body decl)), EA_Ret None p, FunctionResult p) Eb)"
+                 (if falls_through (body decl)
+                  then insert (Statement (m + csize (body decl)), EA_Ret None p, FunctionResult p) Eb
+                  else Eb)"
     by (rule compile_procE)
-  have Ebsub: "Eb \<subseteq> intra ?g" using Edef Esub by auto
+  have Ebsub: "Eb \<subseteq> intra ?g" using Edef Esub by (auto split: if_splits)
   have ent: "(FunctionEntry p, EA_Nop, Statement m) \<in> intra ?g" using Edef Esub by auto
-  have ext: "(Statement (m + csize (body decl)), EA_Ret None p, FunctionResult p) \<in> intra ?g"
+  have ext: "falls_through (body decl) \<longrightarrow>
+               (Statement (m + csize (body decl)), EA_Ret None p, FunctionResult p) \<in> intra ?g"
     using Edef Esub by auto
   show "\<exists>k n n' en E K. compile \<Pi> p (body decl) k n = (n', en, E, K)
           \<and> E \<subseteq> intra ?g \<and> K \<subseteq> calls ?g
           \<and> (FunctionEntry p, EA_Nop, en) \<in> intra ?g
-          \<and> (k, EA_Ret None p, FunctionResult p) \<in> intra ?g
+          \<and> (falls_through (body decl) \<longrightarrow>
+               (k, EA_Ret None p, FunctionResult p) \<in> intra ?g)
           \<and> source_com (body decl)"
     using cb Ebsub Ksub ent ext srccom by blast
+
 qed
 
 end
